src/tls/TLS.Handshake.Client.fst
@@ -9,13 +9,16 @@ open TLS.Handshake.Machine
 
 module B = LowStar.Buffer // not FStar.Bytes
 module CH = Parsers.ClientHello
-module E = Extensions
+// module E = Extensions
 module Epochs = Old.Epochs
 module HSM = HandshakeMessages
+module PF = TLS.Handshake.ParseFlights // avoidable?
 module HMAC = Old.HMAC.UFCMA
 module KS = Old.KeySchedule
 module HS = FStar.HyperStack
-module H = Hashing.Spec
+// module H = Hashing.Spec
+module Transcript = HSL.Transcript
+module Receive = TLS.Handshake.Receive
 
 #set-options "--admit_smt_queries true"
 
@@ -59,29 +62,32 @@ let export #region #n epochs xk =
   FStar.Monotonic.Seq.i_write_at_end epochs.Epochs.exporter xk
 
 
-(*** Version-agnostic messages ***)
+// high-level transcript; floating
+// TODO add precise type & move to Transcript
+let transcript_extract #ha (di:Transcript.state ha) tx: St Bytes.bytes =
+  let ltag = EverCrypt.Hash.Incremental.hash_len ha in
+  let btag = LowStar.Buffer.alloca 0uy ltag in
+  Transcript.extract_hash di btag tx;
+  FStar.Bytes.of_buffer ltag btag
 
+(*** Hello messages ***)
 
 (*
-type btag (binderKey:(i:HMAC.binderId & bk:KS.binderKey i)) =
-  HMAC.tag (HMAC.HMAC_Binder (let (|i,_|) = binderKey in i))
-
-private let compute_binder hs (bkey:(i:HMAC.binderId & bk:KS.binderKey i))
-  : ST (btag bkey)
-  (requires fun h0 -> True)
-  (ensures fun h0 _ h1 -> modifies_none h0 h1) =
-  let (| bid, bk |) = bkey in
-  let digest_CH0 = HSL.hash_tag #(binderId_hash bid) hs.log in
-  HMAC.mac bk digest_CH0
-
 val map_ST2: 'c -> ('c -> 'a -> KS.ST0 'b) -> list 'a -> KS.ST0 (list 'b)
 let rec map_ST2 env f x = match x with
   | [] -> []
   | a::tl -> f env a :: map_ST2 env f tl
-*)
 
+type btag (binderKey:(i:HMAC.binderId & bk:KS.binderKey i)) =
+  HMAC.tag (HMAC.HMAC_Binder (let (|i,_|) = binderKey in i))
 
-(*
+private let compute_binder (bkey:(i:HMAC.binderId & bk:KS.binderKey i)) tag
+  : ST (btag bkey)
+  (requires fun h0 -> True)
+  (ensures fun h0 _ h1 -> modifies_none h0 h1) =
+  let _,bk = bkey in
+  HMAC.mac bkey tag
+
 let client_Binders #region (hs:t region) (offer:HSM.clientHello) =
   match snd hs.cfg with
   | (_, []) ->
@@ -93,26 +99,63 @@ let client_Binders #region (hs:t region) (offer:HSM.clientHello) =
     let binders = map_ST2 hs compute_binder binderKeys in
     let bb = PSK.offeredPsks_binders_serializer32 binders in
     HSL.send_raw hs.log bb;
-
     // Nego ensures that EDI is not sent in a 2nd ClientHello
  *)
 
-let transcript_extract #ha (di:HSL.Transcript.state ha) tx: St Bytes.bytes =
-  let ltag = EverCrypt.Hash.Incremental.hash_len ha in
-  let btag = LowStar.Buffer.alloca 0uy ltag in
-  HSL.Transcript.extract_hash di btag tx;
-  FStar.Bytes.of_buffer ltag btag
+/// Create a transcript digest for the truncated client Hello.
+let client_transcript (region:rgn) ha tch =
+  let di, transcript0 = Transcript.create region ha in
+  let transcript1 = Transcript.extend di (admit() (*of tch*)) transcript0 in
+  let tag = transcript_extract di transcript1 in
+  (tag, di)
 
-/// Create a fresh transcript digest, hash the truncated client Hello,
-/// and compute the MAC for a given PSK.
-//TODO tch & logical payload
-let client_Binder region (bkey:Negotiation.bkey13) tch =
-  let ha = Negotiation.ha_bkey13 bkey in
-  let di, tx0 = HSL.Transcript.create region ha in
-  let tx1 = HSL.Transcript.extend di tch tx0 in
-  let tag = transcript_extract di tx1 in
-  let binder = KS.mk_binder #region bkey in // vs HMAC.mac bk tag, hiding tricky indexing
-  tx1, ha, di, binder
+let btag (bkey:Negotiation.bkey13) =
+  Bytes.bytes
+  // Hacl.Hash.Definitions.hash_t (Negotiation.ha_bkey13 bkey)
+
+// TODO sort it out within KeySchedule
+assume val compute_binder:
+  bkey:Negotiation.bkey13 ->
+  tag: btag bkey -> btag bkey
+
+/// Compute binder MACs for the PSKs; in rare cases we allocate an
+/// auxiliary transcripts for other hash algorithms.
+//TODO type; tch & logical payload
+val client_Binders:
+  region:rgn ->
+  ha0: EverCrypt.Hash.Incremental.alg ->
+  di: Transcript.state ha0 ->
+  tch: full_offer ->
+  bkey: list Negotiation.bkey13 ->
+  ST Bytes.bytes
+  (requires fun h0 ->
+    Transcript.invariant di (transcript_tch tch) h0)
+  (ensures fun h0 b h1 ->
+    modifies_none h0 h1)
+
+let rec client_Binders region ha0 di0 tch bkeys =
+  match bkeys with
+  | [] -> Bytes.empty_bytes
+  | bkey::bkeys ->
+    let ha = Negotiation.ha_bkey13 bkey in
+    let tx: Transcript.g_transcript_n (Ghost.hide 0) = Ghost.hide (transcript_tch tch) in
+    let tag =
+      if ha = ha0 then
+        transcript_extract di0 tx
+      else
+        let tag, di = client_transcript region ha tch in
+        // TODO Transcript.free di
+        tag in
+    let binder = compute_binder bkey tag in
+    Bytes.append binder (client_Binders region ha0 di0 tch bkeys )
+
+let initial_ha offer =
+  match offer.Parsers.ClientHello.cipher_suites with
+  | [] -> EverCrypt.Hash.Incremental.SHA2_256
+  | cs::_ ->
+    match cipherSuite_of_name cs with
+    | Some (CipherSuite.CipherSuite13 _ ha) -> ha
+    | _ -> EverCrypt.Hash.Incremental.SHA2_256
 
 let client_ClientHello (Client region config r) =
   let (cfg,resume) = config in
@@ -127,62 +170,61 @@ let client_ClientHello (Client region config r) =
 
   // Compute & send the ClientHello offer
   // lower: we'll instead pass the sending state for writing the offer.
-  // TODO allocate non-empty output slice!
-  let sending = Send.send_state0 in
   match Negotiation.client_ClientHello config random shares with
   | Error z -> Error z
   | Correct offer0 -> (
-    let epochs = Epochs.create region random in
-    let receiving_buffer = LowStar.Buffer.alloca 0uy 12000ul in
-    let receiving = TLS.Handshake.Receive.create receiving_buffer in
-
-    // TODO: write CH, including dummy binders if it offers PSKs.
-    // Send.send_ch sending offer;
+    let full_offer = {full_retry = None; full_ch = offer0} in
+    // TODO: output CH, including dummy binders if it offers PSKs (no transcript yet)
+    // Send.send_tch sending offer0;
 
     // TODO assert we have a slice with this serialized offer
 
-    // TODO: postcondition stating the transcript is at [ClientHello None offer1], and computing ha from offer1 too
-    let (| offer1, ha, digest |) : (_ & ha:_ & HSL.Transcript.state ha) = (
-      match resume with
-      | (_,[]) -> (
-        let ha = EverCrypt.Hash.Incremental.SHA2_256 in // a reasonable default
-        let di, tx0 = HSL.Transcript.create region ha in
-        let tx1 = HSL.Transcript.(extend di (admit()) (* LR_ClientHello of offer *) tx0) in
-        (| offer0, ha, di |) )
-
-      | (_,(psk0::psks)) -> (
-        // TODO intermediate write to hs for witnessing the binder's
-        // logical payload; this requires a dummy digest.
-        let tx1, ha, di, binder = client_Binder region psk0 (admit()) (* LR_TCH of offer *) in
-        // TODO iterate on the other binders [psks], deallocating their auxiliary digests
-        // TODO patch both the offer and its serialization in [sending]
-        let offer1 = offer0 in
-        let tx2 = HSL.Transcript.(extend di (admit()) (* LR_CompleteTCH of [binder] *) tx1) in
-        let sending =
-        if Negotiation.find_early_data offer0 then (
-          trace "setting up 0RTT";
-          let digest_CH = transcript_extract di tx2  in
-          // TODO consider doing export & register within KS
-          let early_exporter_secret, edk = KS.ks_client13_ch cfg.is_quic ks digest_CH in
-          export epochs early_exporter_secret;
-          register epochs edk;
-          Send.signals sending (Some (true, false)) false )
-        else sending in
-        (| offer1, ha, di |))) in
-
+    // allocate digest state with a reasonable default hash algorithm
+    let ha = initial_ha offer0 in
+    let tag, di = client_transcript region ha offer0 in
+    let tx_tch = Ghost.hide (transcript_tch full_offer) in
+    let sending = Send.send_state0 in
+    let receiving = Receive.(create (alloc_slice region)) in
+    let epochs = Epochs.create region random in
     let ms: msg_state region ParseFlights.F_c_wait_ServerHello random ha = {
-      digest = digest;
+      digest = di;
       sending = sending;
       receiving = receiving;
       epochs = epochs;
     } in
+    // write transient state for witnessing offer0 (used for binders)
+    r := C_wait_ServerHello ({full_retry=None; full_ch=offer0}) ms ks;
+
+    // TODO below: postcondition stating the transcript is at [ClientHello None offer1], and computing ha from offer1 too
+    let (| offer1, ha, digest |) : (_ & ha:_ & Transcript.state ha) = (
+      match resume with
+      | (_,[]) -> (| offer0, ha, di |)
+      | (_,psks) -> (
+        let binders = client_Binders region ha di full_offer psks in
+
+        // TODO patch both the offer and its serialization in [sending]
+        let offer1 = offer0 in
+        let tx1 = Transcript.(extend di (admit()) (* LR_CompleteTCH of [binder] *) tx_tch) in
+        let sending =
+          if Negotiation.find_early_data offer0 then (
+            trace "setting up 0RTT";
+            let digest_CH = transcript_extract di tx1  in
+            // TODO consider doing export & register within KS
+            let early_exporter_secret, edk = KS.ks_client13_ch cfg.is_quic ks digest_CH in
+            export epochs early_exporter_secret;
+            register epochs edk;
+            Send.signals sending (Some (true, false)) false )
+          else sending in
+        (| offer1, ha, di |))) in
+
     r := C_wait_ServerHello ({full_retry=None; full_ch=offer1}) ms ks;
     Correct () )
 
-let client_HelloRetryRequest hs hrr =
+let client_HelloRetryRequest (Client region config r) hrr =
+  let C_wait_ServerHello offer ms ks = !r in
   let open Parsers.HelloRetryRequest in
-  trace("Got HRR, extensions: " ^ Nego.string_of_hrres hrr.extensions);
-  let ch1 = Nego.getOffer hs.nego in
+  trace("HelloRetryRequest with extensions " ^ Nego.string_of_hrres hrr.extensions);
+  let ch1 = offer.full_ch in
   let share, ks =
   match Negotiation.group_of_hrr hrr with
   | None ->
@@ -195,8 +237,8 @@ let client_HelloRetryRequest hs hrr =
       Some (| g, s |), ks
   in
   match Nego.client_HelloRetryRequest ch1 hrr share with
-  | Error z -> InError z
-  | Correct (hri, ch2) ->
+  | Error z -> Receive.InError z
+  | Correct ch2 ->
     // TODO: adapt from the code above
     // does it make sense to send binders with the wrong hash algorithm?
 
@@ -235,30 +277,33 @@ let client_ServerHello (Client region config r) sh =
   trace "client_ServerHello";
   let cfg,_ = config in
   let C_wait_ServerHello offer ms ks = !r in
-  match Negotiation.client_accept_ServerHello config offer.full_ch sh with
+  match Negotiation.client_accept_ServerHello cfg offer.full_ch sh with
   | Error z -> Receive.InError z
   | Correct (cs,pski) -> (
     match cs with
     | CipherSuite13 ae ha -> (
       trace "Running TLS 1.3";
       let server_share = Negotiation.find_serverKeyShare sh in
-      let digest_ServerHello = HSL.hash_tag #ha s.log in
+      let transcript_sh = Transcript.extend ms.digest (admit() (*sh*)) (Ghost.hide (transcript_offer offer)) in
+      //assert(transcript_sh == transcript13 offer sh []);
+      let digest_ServerHello = transcript_extract ms.digest transcript_sh in
       let hs_keys, ks = KS.ks_client13_sh
-        s.ks
+        region
+        ks
         cfg.is_quic
-        sh.RealServerHello.random
+        sh.Parsers.RealServerHello.random
         (CipherSuite13 ae ha)
         digest_ServerHello
         server_share
         pski in
-      register sms.epochs hs_keys; // register new epoch
-      if Negotiation.zeroRTToffer offer.full_ch then (
+      register ms.epochs hs_keys; // register new epoch
+      if Negotiation.find_early_data offer.full_ch then (
         // Skip the 0-RTT epoch on the reading side
-        Epochs.incr_reader s.epochs;
-        match mode.Negotiation.n_pski with
+        Epochs.incr_reader ms.epochs;
+        match pski with
         | None ->
           trace "0-RTT rejected early (no PSK was selected)";
-          Epochs.incr_writer s.epochs
+          Epochs.incr_writer ms.epochs
         | Some _ ->
           trace "0RTT potentially accepted (wait for EE to confirm)";
           // No EOED in QUIC, so we immediately enable HSK
@@ -267,213 +312,229 @@ let client_ServerHello (Client region config r) sh =
         Epochs.incr_writer ms.epochs; // Next flight (CFin) will use HSK
 
       Epochs.incr_reader ms.epochs; // Client 1.3 HSK switch to handshake key for decrypting EE etc...
+      // assume(
+      //   selected_ha sh == offered_ha offer.full_ch /\
+      //   PF.length_parsed_bytes ms.receiving.Receive.pf_st == 0
+      //   );
+      // let ms: msg_state region PF.F_c_wait_ServerHello (offer.full_ch.HSM.random) (selected_ha sh) = ms in
+      // let ms: msg_state region PF.F_c13_wait_Finished1 (offer.full_ch.HSM.random) (selected_ha sh) = {ms with receiving = ms.receiving } in
+      let ms = { ms with receiving = ms.receiving } in
       r := C13_wait_Finished1 offer sh ms ks;
       Receive.InAck true false // Client 1.3 HSK
     )
     | CipherSuite kex sa ae -> (
       trace "Running classic TLS";
-      trace ("Offered SID="^(Bytes.print_bytes mode.Negotiation.n_offer.CH.session_id)^" Server SID="^(Bytes.print_bytes mode.Negotiation.n_sessionID));
-      if Negotiation.resume_12 mode then
-      begin // 1.2 resumption
-        trace "Server accepted our 1.2 ticket.";
-        let Some (tid, Ticket.Ticket12 pv cs ems msId ms) = fst (Negotiation.resume s.nego) in
-        let pv' = mode.Negotiation.n_protocol_version in
-        let cs' = mode.Negotiation.n_cipher_suite in
-        let sr = mode.Negotiation.n_server_random in
-        let nst = Negotiation.sendticket_12 mode in
-        if pv = pv' && cs = cs' then // TODO check full session
-        begin
-          let adk = KS.ks_client12_resume s.ks sr pv cs ems msId ms in
-          let digestSH = HSL.hash_tag #ha s.log in
-          register s adk;
-          s.state := (if nst then C_wait_NST true else C_wait_CCS (true, digestSH));
-          InAck false false
-        end
-        else
-          InError (fatalAlert Handshake_failure, "inconsistent protocol version or ciphersuite during resumption")
-      end
-      else
-      begin // 1.2 full handshake
-        s.state := C_wait_ServerHelloDone;
-        InAck false false
-      end ))
+      trace ("Offered SID="^(Bytes.print_bytes offer.full_ch.CH.session_id)^" Server SID="^(Bytes.print_bytes sh.Parsers.RealServerHello.session_id));
+      Receive.InError (fatalAlert Handshake_failure, "TLS 1.2 TBC")
+      // if Negotiation.resume_12 mode then
+      // begin // 1.2 resumption
+      //   trace "Server accepted our 1.2 ticket.";
+      //   let Some (tid, Ticket.Ticket12 pv cs ems msId ms) = fst (Negotiation.resume s.nego) in
+      //   let pv' = mode.Negotiation.n_protocol_version in
+      //   let cs' = mode.Negotiation.n_cipher_suite in
+      //   let sr = mode.Negotiation.n_server_random in
+      //   let nst = Negotiation.sendticket_12 mode in
+      //   if pv = pv' && cs = cs' then // TODO check full session
+      //   begin
+      //     let adk = KS.ks_client12_resume s.ks sr pv cs ems msId ms in
+      //     let digestSH = HSL.hash_tag #ha s.log in
+      //     register s adk;
+      //     s.state := (if nst then C_wait_NST true else C_wait_CCS (true, digestSH));
+      //     InAck false false
+      //   end
+      //   else
+      //     InError (fatalAlert Handshake_failure, "inconsistent protocol version or ciphersuite during resumption")
+      // end
+      // else
+      // begin // 1.2 full handshake
+      //   s.state := C_wait_ServerHelloDone;
+      //   InAck false false
+      // end
+      ))
 
-let client_ServerHello_HRR s ch1 hri sh =
-  trace "client_ServerHello";
-  match Nego.check_retry ch1 hri sh with
-  | Error z -> InError z
-  | Correct () ->
-    client_ServerHello s sh
-
-(*** TLS 1.2 ***)
-
-private let convert_kex = function
-  | Kex_RSA -> Correct HSM.Rsa
-  | Kex_DHE -> Correct HSM.Dhe
-  | Kex_ECDHE -> Correct HSM.Ecdhe
-  | _ -> fatal Internal_error "Incorrect key exchange selected for 1.2"
-
-let client_ServerHelloDone hs c ske_bytes ocr =
-  trace "processing ...ServerHelloDone";
-  let kex = Negotiation.kexAlg (Negotiation.getMode hs.nego) in
-  match convert_kex kex with
-  | Error z -> InError z
-  | Correct kex ->
-  match HSM.serverKeyExchange_parser32 kex ske_bytes with
-  | None -> InError (fatalAlert Decode_error, "invalid client key exchange")
-  | Some (ske, _) ->
-  match Negotiation.client_ServerKeyExchange hs.nego c kex ske ocr with
-  | Error z -> InError z
-  | Correct mode -> (
-    (match ocr with
-    | None -> ()
-    | Some cr ->
-      trace "processing certificate request (TODO)";
-      HSL.send hs.log (HSL.Msg12 (HSM.M12_certificate [])));
-    let nst = Negotiation.sendticket_12 mode in
-    let gy = Some?.v (mode.Negotiation.n_server_share) in // already set in KS
-    let gx =
-      KS.ks_client12_full_dh hs.ks
-      mode.Negotiation.n_server_random
-      mode.Negotiation.n_protocol_version
-      mode.Negotiation.n_cipher_suite
-      (Negotiation.emsFlag mode) // a flag controlling the use of ems
-      gy in
-    let (|g, _|) = gy in
-    let gxb = CommonDH.serialize_raw gx in
-    let open Parsers.ClientKeyExchange in
-    let cke : clientKeyExchange kex =
-      match kex with
-      | HSM.Ecdhe -> Cke_ecdhe gxb
-      | HSM.Dhe -> Cke_dhe gxb in
-    let msg = HSM.M12_client_key_exchange (
-      clientKeyExchange_serializer32 kex cke) in
-    let ha = verifyDataHashAlg_of_ciphersuite (mode.Negotiation.n_cipher_suite) in
-    let digestClientKeyExchange = HSL.send_tag #ha hs.log (HSL.Msg12 msg) in
-    let cfin_key, app_keys = KS.ks_client12_set_session_hash hs.ks digestClientKeyExchange in
-    register hs app_keys;
-    // we send CCS then Finished;  we will use the new keys only after CCS
-    let cvd = TLSPRF.finished12 ha cfin_key Client digestClientKeyExchange in
-    let fin = HSM.M12_finished cvd in
-    let digestClientFinished = HSL.send_CCS_tag #ha hs.log (HSL.Msg12 fin) false in
-    hs.state := (
-      if nst then
-         C_wait_NST false
-      else
-        C_wait_CCS (false, digestClientFinished));
-    InAck false false)
-
-let client_R_ServerFinished hs f digestNewSessionTicket digestServerFinished =
-  trace "client_R_ServerFinished";
-  let sfin_key = KS.ks12_finished_key hs.ks in
-  let mode = Negotiation.getMode hs.nego in
-  let ha = verifyDataHashAlg_of_ciphersuite mode.Negotiation.n_cipher_suite in
-  let expected_svd = TLSPRF.finished12 ha sfin_key Server digestNewSessionTicket in
-  if f = expected_svd
-  then (
-    let cvd = TLSPRF.finished12 ha sfin_key Client digestServerFinished in
-    let _ = HSL.send_CCS_tag #ha hs.log (HSL.Msg12 (HSM.M12_finished cvd)) true in
-    hs.state := C_Complete; // ADL: TODO need a proper renego state Idle (Some (vd,svd)))};
-    InAck false false // send_CCS_tag buffers the complete
-  )
-  else
-    InError (fatalAlert Decode_error, "Finished MAC did not verify: expected digest "^Bytes.print_bytes digestNewSessionTicket)
-
-let client_ServerFinished hs f digestClientFinished =
-  let sfin_key = KS.ks12_finished_key hs.ks in
-  let mode = Negotiation.getMode hs.nego in
-  let ha = verifyDataHashAlg_of_ciphersuite mode.Negotiation.n_cipher_suite in
-  let expected_svd = TLSPRF.finished12 ha sfin_key Server digestClientFinished in
-  //let expected_svd = TLSPRF.verifyData (mode.Negotiation.n_protocol_version,mode.Negotiation.n_cipher_suite) sfin_key Server digestClientFinished in
-  if f = expected_svd
-  then (
-    hs.state := C_Complete; // ADL: TODO need a proper renego state Idle (Some (vd,svd)))};
-    InAck false true // Client 1.2 ATK
-    )
-  else
-    InError (fatalAlert Decode_error, "Finished MAC did not verify: expected digest "^Bytes.print_bytes digestClientFinished)
-
-let client_NewSessionTicket_12 (hs:hs) (resume:bool) (digest:Hashing.anyTag) (st: HSM.newSessionTicket12)
-  : St incoming =
-  let open Parsers.NewSessionTicket12 in
-  let open TLS.Callbacks in
-  trace ("Processing ticket: "^Bytes.print_bytes st.ticket);
-
-  hs.state := C_wait_CCS (resume, digest);
-  let cfg = Negotiation.local_config hs.nego in
-  let tcb = cfg.ticket_callback in
-  let mode = Negotiation.getMode hs.nego in
-  let Some sni = Bytes.iutf8_opt (Negotiation.get_sni mode.Negotiation.n_offer) in
-
-  let (_msId, ms) = KS.ks12_ms hs.ks in
-  let info = TLS.Callbacks.TicketInfo_12 (
-    mode.Negotiation.n_protocol_version,
-    mode.Negotiation.n_cipher_suite,
-    Negotiation.emsFlag mode) in
-
-  tcb.new_ticket tcb.ticket_context sni st.ticket info ms;
-  InAck false false
+// let client_ServerHello_HRR s ch1 hri sh =
+//   trace "client_ServerHello";
+//   match Nego.check_retry ch1 hri sh with
+//   | Error z -> InError z
+//   | Correct () ->
+//     client_ServerHello s sh
 
 (*** TLS 1.3 ***)
 
-let client_ClientFinished_13 hs digestServerFinished ocr cfin_key =
-  let mode = Negotiation.getMode hs.nego in
-  let ha = verifyDataHashAlg_of_ciphersuite (mode.Negotiation.n_cipher_suite) in
-  let digest =
-    match ocr with
-    | Some cr ->
-      let open Parsers.Certificate13 in
-      let c = ({certificate_request_context = Bytes.empty_bytes; certificate_list = []}) in
-      HandshakeLog.send_tag #ha hs.log (HSL.Msg13 (HSM.M13_certificate c))
-    | None -> digestServerFinished in
-  let (| finId, cfin_key |) = cfin_key in
-  let cvd = HMAC.mac cfin_key digest in
-  let digest_CF = HSL.send_tag #ha hs.log (HSL.Msg13 (HSM.M13_finished cvd)) in
-  KS.ks_client13_cf hs.ks digest_CF; // For Post-HS
-  Epochs.incr_reader hs.epochs; // to ATK
-  HSL.send_signals hs.log (Some (true, false)) true; //was: Epochs.incr_writer hs.epochs
-  hs.state := C_Complete // full_mode (cvd,svd); do we still need to keep those?
+let client13_Finished2 (Client region config r) (*ocr*) =
 
-let client_ServerFinished_13 hs ee ocr oc ocv
-  svd digestCert digestCertVerify digestServerFinished =
-  let oc =
-    let open Parsers.Certificate13 in
-    match oc with | None -> None | Some c -> Some c.certificate_list in
-  let cfg = Negotiation.local_config hs.nego in
-  match Negotiation.clientComplete_13 hs.nego ee ocr oc ocv digestCert with
-  | Error z -> InError z
-  | Correct mode ->
-    // ADL: 4th returned value is the exporter master secret.
-       // should be passed to application somehow --- store in Nego? We need agreement.
-       let (sfin_key, cfin_key, app_keys, exporter_master_secret) = KS.ks_client13_sf hs.ks digestServerFinished in
-       let (| finId, sfin_key |) = sfin_key in
-       if not (HMAC.verify sfin_key digestCertVerify svd)
-       then InError (fatalAlert Decode_error, "Finished MAC did not verify: expected digest "^Bytes.print_bytes digestCertVerify )
-       else
-       begin
-         export hs exporter_master_secret;
-         register hs app_keys; // ATKs are ready to use in both directions
+  let C13_complete offer sh ee server_id fin1 fin2 eoed_args ms ks = !r in
+  let ha = selected_ha sh in
+  let hlen = Hacl.Hash.Definitions.hash_len ha in
+  let btag: Hacl.Hash.Definitions.hash_t ha = B.alloca 0uy 64ul in // large enough for any digest
 
-         // EOED emitting (not used for QUIC)
-         if Negotiation.zeroRTT mode && not cfg.is_quic then
-         begin
-           trace "Early data accepted; emitting EOED.";
-           let ha = Negotiation.hashAlg mode in
-           let digestEOED = HSL.send_tag #ha hs.log (HSL.Msg13 (HSM.M13_end_of_early_data ())) in
-           HSL.send_signals hs.log (Some (false, false)) false;
-           hs.state := C13_sent_EOED digestEOED ocr cfin_key;
-           InAck false false
-         end
-         else
-         begin
-           (if Negotiation.zeroRTT mode then trace "Early data accepted (QUIC, no EOED)."
-           else trace "Early data rejected");
-           client_ClientFinished_13 hs digestServerFinished ocr cfin_key;
-           InAck true false // Client 1.3 ATK; next the client will read again to send Finished, writer++, and the Complete signal
-         end
-       end // moving to C_Complete
+  // TODO: support certificate-based client authentication
+  // let digest =
+  //   match ocr with
+  //   | Some cr ->
+  //     let open Parsers.Certificate13 in
+  //     let c = ({certificate_request_context = Bytes.empty_bytes; certificate_list = []}) in
+  //     HandshakeLog.send_tag #ha hs.log (HSL.Msg13 (HSM.M13_certificate c))
+  //   | None -> digestServerFinished in
 
-let c13_NewSessionTicket hs st13 =
+  // prepare & send Finished2
+  let transcript_Finished1: Transcript.g_transcript_n (Ghost.hide 0) = Ghost.hide (transcript13 offer sh []) in
+  Transcript.extract_hash ms.digest btag transcript_Finished1;
+  let digest_Finished1 = Bytes.of_buffer hlen btag in
+
+  // to be updated, possibly using btag as output buffer.
+  // may use an abstract accessor instead: (i:HMAC.finishedId & cfk:KS.fink i)
+  let Old.KeySchedule.C13_wait_Finished2 _ (| cfin_id, cfin_key |) _ _ = ks in
+  let cvd = HMAC.mac cfin_key digest_Finished1 in
+  let fin2 = Ghost.hide #finished cvd in
+
+  match Send.send_tag13 ms.digest transcript_Finished1 ms.sending (HSM.M13_finished cvd) btag with
+  | Error z -> Error z
+  | Correct (sending, transcript_Finished2) ->
+
+  let digest_Finished2 = FStar.Bytes.of_buffer hlen btag in
+  let ks = KS.ks_client13_cf ks digest_Finished2 in // post-handshake keying
+  Epochs.incr_reader ms.epochs; // to ATK
+  let sending = Send.signals sending (Some (true, false)) true in
+
+  let ms = { ms with sending = sending } in
+  // updating [ms.sending fin2 ks]
+  r := C13_complete offer sh ee server_id fin1 fin2 eoed_args ms ks;
+  Correct ()
+
+let client13_nego_cb cfg ee =
+  trace ("Received encrypted extensions "^Negotiation.string_of_ees ee);
+  trace ("Negotiation callback to process application extensions.");
+  let uexts = List.Tot.filter Parsers.EncryptedExtension.EE_Unknown_extensionType? ee in
+  // the length check below could be statically excluded from the definition of filtering
+  if not (Parsers.EncryptedExtensions.check_encryptedExtensions_list_bytesize uexts)
+  then
+    fatal Internal_error "encrypted extensions are too large"
+  else
+  let uexts_bytes = Parsers.EncryptedExtensions.encryptedExtensions_serializer32 uexts in
+  // to be simplified (see TLS.Callbacks)
+  let cb = cfg.nego_callback in
+  let open TLS.Callbacks in
+  match cb.negotiate cb.nego_context TLS_1p3 uexts_bytes None with
+  | Nego_abort    -> fatal Handshake_failure "application requested to abort the handshake"
+  | Nego_retry _  -> fatal Internal_error "client application requested a server retry"
+  | Nego_accept _ -> Correct ()
+
+// annoying differently refined bytes, to be reviewed
+type cert_repr = Parsers.ASN1Cert.aSN1Cert // aka b:bytes {length b < 16777216} but with another syntax
+private let coerce_asncert (x:Parsers.ASN1Cert.aSN1Cert): cert_repr = x
+private let coerce_crt crt = List.Tot.map coerce_asncert crt
+
+// process the certificate chain and verify the server signature
+let client13_c_cv cfg offer ha transcript_ee (digest: Transcript.state ha)
+  (c: HSM.certificate13)
+  (cv: HSM.certificateVerify13) =
+  let transcript_c = Transcript.extend digest (admit()(*c*)) transcript_ee in
+  let digest_signed = transcript_extract digest transcript_c in
+  let transcript_cv = Transcript.extend digest (admit()(*cv*)) transcript_c in
+
+  // TODO ensure that valid_offer mandates signature extensions for 1.3
+  let sal = match Negotiation.find_signature_algorithms offer with
+  | Some sal -> sal
+  | None -> [] in
+    let sa = cv.HSM.algorithm in
+    let chain = Some (c, sa) in
+    if not (List.Tot.mem sa sal)
+    then
+      fatal Bad_certificate "The server signed with an algorithm we did not offer"
+    else
+      let tbs = Negotiation.to_be_signed TLS_1p3 TLSConstants.Server None digest_signed in
+      let chain = coerce_crt (Cert.chain_down c.HSM.certificate_list) in
+      if not (TLS.Callbacks.cert_verify_cb cfg.cert_callbacks chain sa tbs cv.HSM.signature)
+      then (
+        trace("Certificate & signature 1.3 callback failed");
+        fatal Bad_certificate "Failed to validate signature or certificate" )
+      else (
+        trace("Certificate & signature 1.3 callback succeeded");
+        Correct transcript_cv )
+
+let client13_Finished1 hs ee client_cert_request server_cert_certverify finished
+=
+  let Client region (cfg,_) r = hs in
+  match client13_nego_cb cfg ee with
+  | Error z -> Receive.InError z
+  | Correct _ ->
+  match client_cert_request with
+  | Some _ -> Receive.InError (fatalAlert Handshake_failure,"unsupported client certificate request")
+  | None ->
+
+  let C13_wait_Finished1 offer sh ms ks = !r in
+  let ha = selected_ha sh in
+  let hlen = Hacl.Hash.Definitions.hash_len ha in
+  let btag: Hacl.Hash.Definitions.hash_t ha = B.alloca 0uy 64ul in // large enough for any digest
+  let transcript_ee: Ghost.erased Transcript.transcript_t = Transcript.extend ms.digest
+    (admit()(* LR for ee *))
+    (Ghost.hide (transcript13 offer sh [])) in
+  let psk_based = Some? (Negotiation.find_serverPske sh) in
+  let verified_server =
+    match server_cert_certverify with
+    | None ->
+        if not psk_based then
+          fatal Handshake_failure "missing certificate chain and sigature"
+        else
+          // relying on a previously received & verified server
+          // certificate chain & signature recorded for this PSK; TODO
+          // confirm this context is available to the application.
+          Correct transcript_ee
+
+    | Some (c,cv) ->
+        if psk_based then
+          fatal Handshake_failure "unexpected certificate chain and signature"
+        else
+          client13_c_cv cfg offer.full_ch ha transcript_ee ms.digest c cv
+  in
+  match verified_server with
+  | Error z -> Receive.InError z
+  | Correct transcript_maced -> (
+    // let oc =
+    // let open Parsers.Certificate13 in
+    // match oc with | None -> None | Some c -> Some c.certificate_list in
+    // let cfg = Negotiation.local_config hs.nego in
+    // match Negotiation.clientComplete_13 hs.nego ee ocr oc ocv digestCert with
+
+  let digest_maced = transcript_extract ms.digest transcript_maced in
+  let transcript_Finished1 = Transcript.(extend ms.digest (admit()(*finished*)) transcript_maced) in
+  let digest_Finished1 = transcript_extract ms.digest transcript_Finished1 in
+  let ks, (sfin_key, cfin_key, app_keys, exporter_master_secret) = KS.ks_client13_sf cfg.is_quic ks digest_Finished1 in
+  // ADL: 4th returned value is the exporter master secret.
+  // should be passed to application somehow --- store in Nego? We need agreement.
+
+  let (| finId, sfin_key |) = sfin_key in
+  if not (HMAC.verify sfin_key digest_maced digest_maced)
+  then
+    Receive.InError (fatalAlert Decode_error, "Finished MAC did not verify: expected digest "^Bytes.print_bytes digest_maced)
+  else (
+    export ms.epochs exporter_master_secret;
+    register ms.epochs app_keys; // ATKs are ready to use in both directions
+
+    if Negotiation.zeroRTT sh && not cfg.is_quic // EOED emitting (not used for QUIC)
+    then (
+      trace "Early data accepted; emitting EOED.";
+      match Send.send13 #ha ms.digest #(Ghost.hide 0) (admit()) ms.sending (HSM.M13_end_of_early_data ()) with
+      | Correct (sending, transcript) -> (
+        let sending = Send.signals sending (Some (false, false)) false in
+        let eoed_args = Some (None, cfin_key) in
+        let fin1 = Ghost.hide Bytes.empty_bytes in
+        let fin2 = Ghost.hide Bytes.empty_bytes in
+        r := C13_complete offer sh ee server_cert_certverify fin1 fin2 eoed_args ms ks; // digestEOED ocr cfin_key;
+        Receive.InAck false false )
+      | Error z -> Receive.InError z )
+    else (
+      (if Negotiation.zeroRTT sh
+      then trace "Early data accepted (QUIC, no EOED)."
+      else trace "Early data rejected");
+      // TODO write r before this call!
+      match client13_Finished2 hs with
+      | Error z   -> Receive.InError z
+      | Correct _ -> Receive.InAck true false // Client 1.3 ATK; next the client will read again to send Finished, writer++, and the Complete signal
+      )))
+
+let client13_NewSessionTicket (Client region config r) st13 =
   let open TLS.Callbacks in
   let open Parsers.NewSessionTicket13 in
   let open Parsers.NewSessionTicketExtension in
@@ -482,26 +543,26 @@ let c13_NewSessionTicket hs st13 =
   let age_add = st13.ticket_age_add in
   trace ("Received ticket: "^Bytes.hex_of_bytes tid^" nonce: "^Bytes.hex_of_bytes nonce);
 
-  match !hs.state with
-  | C13_complete offer sh ee server_id _fin1 _fin2 _eoed_args _ms ks ->
-    let cs = sh.RealServerHello.cipher_suite in
-    let ed = List.Tot.find NSTE_early_data? st13.extensions in
-    let now = UInt32.uint_to_t (FStar.Date.secondsFromDawn()) in
-    let info = TicketInfo_13 TLS.Callbacks.({
-      ticket_nonce = Some nonce;
-      time_created = now;
-      ticket_age_add = age_add;
-      allow_early_data = Some? ed;
-      allow_dhe_resumption = true;
-      allow_psk_resumption = true;
-      early_cs = cs;
-      identities = (Bytes.empty_bytes, Bytes.empty_bytes); // TODO certs
-    }) in
+  let C13_complete offer sh ee server_id _fin1 _fin2 _eoed_args _ms ks = !r in
+  let cs = sh.Parsers.RealServerHello.cipher_suite in
+  let Some cs = CipherSuite.cipherSuite_of_name cs in // add static refinement?
+  let ed = List.Tot.find NSTE_early_data? st13.extensions in
+  let now = UInt32.uint_to_t (FStar.Date.secondsFromDawn()) in
+  let info = TicketInfo_13 TLS.Callbacks.({
+    ticket_nonce = Some nonce;
+    time_created = now;
+    ticket_age_add = age_add;
+    allow_early_data = Some? ed;
+    allow_dhe_resumption = true;
+    allow_psk_resumption = true;
+    early_cs = cs;
+    identities = (Bytes.empty_bytes, Bytes.empty_bytes); // TODO certs
+  }) in
 
-    let psk = KS.ks_client13_rms_psk ks nonce in
-    let Some sni = Bytes.iutf8_opt (Negotiation.get_sni offer.full_ch) in
-    let cfg = fst hs.cfg in
-    let valid_ed =
+  let psk = KS.ks_client13_rms_psk ks nonce in
+  let Some sni = Bytes.iutf8_opt (Negotiation.get_sni offer.full_ch) in
+  let cfg = fst config in
+  let valid_ed =
     if cfg.is_quic then
       (match ed with
       | None -> true
@@ -511,15 +572,125 @@ let c13_NewSessionTicket hs st13 =
   if valid_ed then
     (let tcb = cfg.ticket_callback in
     tcb.new_ticket tcb.ticket_context sni tid info psk;
-    InAck false false)
+    Receive.InAck false false)
   else
-    InError (fatalAlert Illegal_parameter, "QUIC tickets must allow 0xFFFFFFFF bytes of early data")
+    Receive.InError (fatalAlert Illegal_parameter, "QUIC tickets must allow 0xFFFFFFFF bytes of early data")
 
-
-let early_rejected st =
-  match !st.cstate with
+let early_rejected (Client region config r) =
+  match !r with
   | C13_wait_Finished1 offer sh _ _
   | C13_complete offer sh _ _ _ _ _ _ _ ->
     Negotiation.find_early_data offer.full_ch &&
-    not (List.Tot.existb SHE_early_data? sh.Parsers.RealServerHello.extensions)
+    not (List.Tot.existsb Parsers.ServerHelloExtension.SHE_early_data? sh.Parsers.RealServerHello.extensions)
   | _ -> false
+
+(*** TLS 1.2 ***)
+
+private let convert_kex = function
+  | Kex_RSA -> Correct HSM.Rsa
+  | Kex_DHE -> Correct HSM.Dhe
+  | Kex_ECDHE -> Correct HSM.Ecdhe
+  | _ -> fatal Internal_error "Incorrect key exchange selected for 1.2"
+
+let client12_ServerHelloDone hs c ske_bytes ocr =
+  trace "processing ...ServerHelloDone";
+  Receive.InError (fatalAlert Internal_error, "TBC")
+  // let kex = Negotiation.kexAlg (Negotiation.getMode hs.nego) in
+  // match convert_kex kex with
+  // | Error z -> InError z
+  // | Correct kex ->
+  // match HSM.serverKeyExchange_parser32 kex ske_bytes with
+  // | None -> InError (fatalAlert Decode_error, "invalid client key exchange")
+  // | Some (ske, _) ->
+  // match Negotiation.client_ServerKeyExchange hs.nego c kex ske ocr with
+  // | Error z -> InError z
+  // | Correct mode -> (
+  //   (match ocr with
+  //   | None -> ()
+  //   | Some cr ->
+  //     trace "processing certificate request (TODO)";
+  //     HSL.send hs.log (HSL.Msg12 (HSM.M12_certificate [])));
+  //   let nst = Negotiation.sendticket_12 mode in
+  //   let gy = Some?.v (mode.Negotiation.n_server_share) in // already set in KS
+  //   let gx =
+  //     KS.ks_client12_full_dh hs.ks
+  //     mode.Negotiation.n_server_random
+  //     mode.Negotiation.n_protocol_version
+  //     mode.Negotiation.n_cipher_suite
+  //     (Negotiation.emsFlag mode) // a flag controlling the use of ems
+  //     gy in
+  //   let (|g, _|) = gy in
+  //   let gxb = CommonDH.serialize_raw gx in
+  //   let open Parsers.ClientKeyExchange in
+  //   let cke : clientKeyExchange kex =
+  //     match kex with
+  //     | HSM.Ecdhe -> Cke_ecdhe gxb
+  //     | HSM.Dhe -> Cke_dhe gxb in
+  //   let msg = HSM.M12_client_key_exchange (
+  //     clientKeyExchange_serializer32 kex cke) in
+  //   let ha = verifyDataHashAlg_of_ciphersuite (mode.Negotiation.n_cipher_suite) in
+  //   let digestClientKeyExchange = HSL.send_tag #ha hs.log (HSL.Msg12 msg) in
+  //   let cfin_key, app_keys = KS.ks_client12_set_session_hash hs.ks digestClientKeyExchange in
+  //   register hs app_keys;
+  //   // we send CCS then Finished;  we will use the new keys only after CCS
+  //   let cvd = TLSPRF.finished12 ha cfin_key Client digestClientKeyExchange in
+  //   let fin = HSM.M12_finished cvd in
+  //   let digestClientFinished = HSL.send_CCS_tag #ha hs.log (HSL.Msg12 fin) false in
+  //   hs.state := (
+  //     if nst then
+  //        C_wait_NST false
+  //     else
+  //       C_wait_CCS (false, digestClientFinished));
+  //   InAck false false)
+
+let client12_R_ServerFinished hs f digestNewSessionTicket digestServerFinished =
+  trace "client_R_ServerFinished";
+  Receive.InError (fatalAlert Internal_error, "TBC")
+  // let sfin_key = KS.ks12_finished_key hs.ks in
+  // let mode = Negotiation.getMode hs.nego in
+  // let ha = verifyDataHashAlg_of_ciphersuite mode.Negotiation.n_cipher_suite in
+  // let expected_svd = TLSPRF.finished12 ha sfin_key Server digestNewSessionTicket in
+  // if f = expected_svd
+  // then (
+  //   let cvd = TLSPRF.finished12 ha sfin_key Client digestServerFinished in
+  //   let _ = HSL.send_CCS_tag #ha hs.log (HSL.Msg12 (HSM.M12_finished cvd)) true in
+  //   hs.state := C_Complete; // ADL: TODO need a proper renego state Idle (Some (vd,svd)))};
+  //   InAck false false // send_CCS_tag buffers the complete
+  // )
+  // else
+  //   InError (fatalAlert Decode_error, "Finished MAC did not verify: expected digest "^Bytes.print_bytes digestNewSessionTicket)
+
+let client12_ServerFinished hs f digestClientFinished =
+  Receive.InError (fatalAlert Internal_error, "TBC")
+  // let sfin_key = KS.ks12_finished_key hs.ks in
+  // let mode = Negotiation.getMode hs.nego in
+  // let ha = verifyDataHashAlg_of_ciphersuite mode.Negotiation.n_cipher_suite in
+  // let expected_svd = TLSPRF.finished12 ha sfin_key Server digestClientFinished in
+  // //let expected_svd = TLSPRF.verifyData (mode.Negotiation.n_protocol_version,mode.Negotiation.n_cipher_suite) sfin_key Server digestClientFinished in
+  // if f = expected_svd
+  // then (
+  //   hs.state := C_Complete; // ADL: TODO need a proper renego state Idle (Some (vd,svd)))};
+  //   InAck false true // Client 1.2 ATK
+  //   )
+  // else
+  //   InError (fatalAlert Decode_error, "Finished MAC did not verify: expected digest "^Bytes.print_bytes digestClientFinished)
+
+let client12_NewSessionTicket hs (resume:bool) (digest:Hashing.anyTag) (st: HSM.newSessionTicket12) =
+  let open Parsers.NewSessionTicket12 in
+  let open TLS.Callbacks in
+  trace ("Processing ticket: "^Bytes.print_bytes st.ticket);
+  Receive.InError (fatalAlert Internal_error, "TBC")
+  // hs.state := C_wait_CCS (resume, digest);
+  // let cfg = Negotiation.local_config hs.nego in
+  // let tcb = cfg.ticket_callback in
+  // let mode = Negotiation.getMode hs.nego in
+  // let Some sni = Bytes.iutf8_opt (Negotiation.get_sni mode.Negotiation.n_offer) in
+
+  // let (_msId, ms) = KS.ks12_ms hs.ks in
+  // let info = TLS.Callbacks.TicketInfo_12 (
+  //   mode.Negotiation.n_protocol_version,
+  //   mode.Negotiation.n_cipher_suite,
+  //   Negotiation.emsFlag mode) in
+
+  // tcb.new_ticket tcb.ticket_context sni st.ticket info ms;
+  // InAck false false
