src/tls/Negotiation.fsti
@@ -2,9 +2,6 @@ module Negotiation
 
 /// Negotiates the TLS parameters for connection establishment,
 /// based on the local configuration and the peer's hello message.
-///
-/// Defines datatypes holding the TLS parameters: [offer] and [mode]
-/// used in Handshake, FFI, QUIC.
 
 // What's an appropriate abstraction for this interface? Provide both
 // pure specs and the supporting state machine? Keep offer and mode
@@ -39,7 +36,9 @@ val print_namedGroupList
   (ensures (fun h _ h' -> B.modifies B.loc_none h h'))
 
 val string_of_hrres: Parsers.HRRExtensions.hRRExtensions -> string
+val string_of_ees: Parsers.EncryptedExtensions.encryptedExtensions -> string
 
+// duplicating Negotiation.Version, for visibility 
 let implemented_version = pv:protocolVersion {pv = TLS_1p2 || pv = TLS_1p3}
 
 type pre_share = g:CommonDH.group & CommonDH.pre_share g
@@ -47,21 +46,16 @@ type share = g:CommonDH.group & CommonDH.share g
 
 let offer = HSM.clientHello
 
-(*
-  After issuing/receiving the second ClientHello, 
-  we keep both the server's HelloRetryRequest
-  and the overwritten parts of the initial offer.
-*)
-type retryInfo (offer:offer) =
-  HSM.hrr *
-  list pre_share (* we should actually keep the raw client extension content *) *
-  list Extensions.pskIdentity
-
+val find_signature_algorithms: offer -> option signatureSchemeList
 val find_cookie: offer -> option Extensions.cookie 
 val find_psk_key_exchange_modes: offer -> list Extensions.pskKeyExchangeMode // [] when not found; pick better representation?
 val find_sessionTicket: offer -> option Extensions.clientHelloExtension_CHE_session_ticket 
 val find_clientPske: offer -> option Extensions.offeredPsks 
 val find_serverKeyShare: HSM.sh -> option pre_share 
+val find_serverPske: HSM.sh -> option UInt16.t
+(* Returns the server hostName, if any, or an empty bytestring; review. *)
+val get_sni: offer -> Tot bytes 
+
 
 // the type of correct indexes into the list of PSKs offered by the client
 type pski (o:offer) = n:nat {
@@ -78,12 +72,13 @@ type cr =
 | CertRequest12 of HSM.certificateRequest12
 | CertRequest13 of HSM.certificateRequest13
 
-(**
+(*
   The final negotiated outcome, including key shares and long-term identities.
   mode is the name used in the resilience paper;
   session_info is the one from TLSInfo
-*)
+
 // can we make it abstract? get rid of accessor functions? used directly in Handshake. 
+//19-08-30 deprecated
 noeq type mode =
   | Mode:
     n_offer: offer -> // negotiated client offer
@@ -113,6 +108,7 @@ noeq type mode =
     n_client_share: option share ->
     // { both shares are in the same negotiated group }
     mode
+*)
 
 (* 19-05-28
 // are we better off with a concrete mode? 
@@ -154,12 +150,18 @@ type certNego = option (cert_type * signatureScheme)
 
 val find_early_data: offer -> bool 
 
+(*
+//19-08-30 deprecated
 noeq type negotiationState (r:role) (cfg:config) : Type0 =
   // Have C_Offer_13 and C_Offer? Shares aren't available in C_Offer yet
   | C_Init:     n_client_random: TLSInfo.random ->
                 negotiationState r cfg
 
   | C_Offer:    n_offer: offer ->
+                negotiationState r cfg
+
+  | C_HRR:      n_offer: offer ->
+                n_hrr: retryInfo n_offer ->
                 negotiationState r cfg
 
   | C_WaitFinished1:
@@ -179,6 +181,11 @@ noeq type negotiationState (r:role) (cfg:config) : Type0 =
                 negotiationState r cfg
 
   | S_Init:     n_server_random: TLSInfo.random ->
+                negotiationState r cfg
+
+  // Waiting for ClientHello2
+  | S_HRR:      n_offer: offer ->
+                n_hrr: HSM.hrr ->
                 negotiationState r cfg
 
   | S_ClientHello: // Transitional state to allow Handshake to call KS and generate a share
@@ -224,7 +231,13 @@ type reader 'a =
   (requires (fun h0 -> h0 `HS.contains` ns.state ))
   (ensures (fun h0 _ h1 -> h0 == h1))
 
+// For QUIC, the handshake signals it is returning HRR (to issue a special packet type)
+// val is_server_hrr: reader bool 
+
+// use instead Machine.selected_ha 
 val hashAlg: mode -> Hashing.Spec.alg
+
+
 val kexAlg: mode -> TLSConstants.kexAlg
 val aeAlg:
   m:mode{CipherSuite? m.n_cipher_suite \/ CipherSuite13? m.n_cipher_suite} ->
@@ -259,11 +272,6 @@ val resume:
   #region:rgn -> #role:TLSConstants.role -> t region role -> 
   Tot resumeInfo
 
-val getOffer: reader offer
-val getMode: reader mode
-
-(* Returns the negotiated version, when known, or cfg.max_version *)
-val version: reader protocolVersion 
 
 let footprint
   (#region:rgn) (#role:TLSConstants.role) (ns:t region role)
@@ -275,18 +283,26 @@ let inv (#region:rgn) (#role:TLSConstants.role) (ns:t region role) h0 = h0 `HS.c
 // signature callback; is it used outside Negotiation? 
 // TODO 19-01-06 effect of signing
 val sign: 
-  #region:rgn -> #role:TLSConstants.role -> ns:t region role -> 
+  #region:rgn -> 
+  #role:TLSConstants.role -> 
+  ns:t region role -> 
   bytes -> 
   ST (result HandshakeMessages.certificateVerify13)
   (requires fun h0 -> inv ns h0)
   (ensures fun h0 _ h1 -> inv ns h1)
+*)
 
 
 (* CLIENT *) 
 
 let client_config = config * resumeInfo
 
-/// What the client offers, abstractly. 
+/// What the client offers (spec, eventually noextract).
+///
+/// May fail for unimplemented configurations.
+
+val zeroRTT: HSM.sh -> bool
+
 val client_offer: 
   ccfg: client_config -> 
   nonce:TLSInfo.random -> 
@@ -295,14 +311,15 @@ val client_offer:
 
 /// [C_Init ==> C_Offer]
 ///
-/// [oks] are the optional client key shares sampled by [ks_client_init]
+/// [oks] are the optional client key shares sampled by
+/// [ks_client_init], present when the client offers TLS 1.3 EDH.
 ///
 /// [now] is the current time (an underspecified read effect) used for
-/// age obfuscation; we could also return it ghostly or pass it in
-/// config.
+/// age obfuscation; we could also pass it in config, or return it
+/// ghostly.
 ///
-/// Fails when the version is misconfigurated 
-/// 
+/// Fails when the version is misconfigured 
+
 val client_ClientHello: 
   ccfg: client_config ->
   nonce: TLSInfo.random -> 
@@ -311,26 +328,28 @@ val client_ClientHello:
   (requires fun h0 -> True)  
   (ensures fun h0 r h1 -> 
     B.modifies B.loc_none h0 h1 /\
-    (exists (now:UInt32.t). (r = client_offer ccfg nonce oks now)))
+    (exists (now:UInt32.t). (r == client_offer ccfg nonce oks now)))
 
 // deprecated--use TLS.Cookie.find_keyshare 
 val group_of_hrr: HSM.hrr -> option CommonDH.namedGroup
 
-// Pure spec of computing CH2 from CH1+HRR
+// Pure spec of computing CH2 from CH1 + HRR
 val client_HelloRetryRequest:
   ch1: offer ->
   hrr: HSM.hrr -> 
-  s: share -> 
-  result (retryInfo ch1 & offer)
+  s: option share -> 
+  result offer
 
-// Pure spec of checking retry consistency
+// Pure spec of checking SH is compatible with prior HRR 
 val check_retry:
   ch1: offer ->
-  ri: retryInfo ch1 ->
+  hrr: HSM.hrr -> 
+  ch2: offer -> 
   sh: HSM.sh ->
-  (result unit)
+  result unit
 
-/// What the client accepts, abstractly.
+
+/// What the client accepts (spec, eventually noextract).
 ///
 /// This mode is still partial.
 /// Do we need some spec-level matching with the server's mode?
@@ -341,23 +360,24 @@ val check_retry:
 ///   let client_mode = accept_ServerHello client_cfg offer sh in
 ///   server_mode == client_mode // excluding encrypted extensions, server_cert, etc 
 
-//19-08-20  newer simpler call; the two below will probably go
+
+/// [C_Offer | C_HRR_offer ==> C_Mode] with TODO hrr
+///
+/// Fails if the server's choices are unacceptable
+
 val client_accept_ServerHello: 
   config -> 
   offer: offer -> 
   HSM.sh -> 
   result (cipherSuite * option (pski offer))
 
+(*
 val accept_ServerHello: 
   config -> 
   offer: offer -> 
   HSM.sh -> 
   result (m:mode {m.n_offer == offer})
 
-/// [C_Offer ==> C_Mode]
-///
-/// Fails if the server's choices are unacceptable
-/// 
 val client_ServerHello: 
   #region:rgn -> ns: t region Client ->
   sh: HSM.sh ->
@@ -374,9 +394,10 @@ val client_ServerHello:
       | Correct m0, Correct m1 -> HS.sel h1 ns.state == C_Mode m0 /\ m0 == m1 
       | Error z0, Error z1     -> z0 == z1 
       | _                      -> False))  
+*)
 
-/// Formatting of the server's signed information: called by Handshake
-/// for signing, called by Negotiation for verification,
+/// Formatting the server's signed information: called by Handshake
+/// for signing; called by Negotiation for verification.
 ///
 /// We can implement the two functions separately, but still need
 /// joint injectivity relying on honest nonces never being zero.
@@ -398,9 +419,8 @@ val to_be_signed:
   tbs:bytes {(None? csr <==> pv == TLS_1p3) /\ Bytes.length tbs <= 128} -> 
   bytes
 
-
+(*
 val client_ServerKeyExchange: 
-  #region:rgn -> ns: t region Client ->
   serverCert:HandshakeMessages.certificate12 ->
   kex: Parsers.KeyExchangeAlgorithm.keyExchangeAlgorithm ->
   ske: HandshakeMessages.serverKeyExchange kex ->
@@ -410,21 +430,30 @@ val client_ServerKeyExchange:
   (ensures fun h0 _ h1 -> inv ns h1) 
   // [C_Mode ==> C_Mode] setting [server_share; client_cert_request; server_cert] in mode,
   // requires mode.n_protocol_version = TLS_1p2
+*)
 
 //$ align name to Handshake machine; strengthen post-condition using server Finished1.
+
+/// Process the encrypted server messages:
+/// - calls back for the application for processing unknown extensions (may fail)
+/// - when present, verify server certificate and signature
+/// 
+/// (conversely, the Finished message is verified by Handshake.Client)
+/// 
 val clientComplete_13: 
-  #region:rgn -> ns:t region Client ->
+  // #region:rgn -> ns:t region Client ->
+  config -> 
+  offer -> 
+  kexAlg -> 
   ee: HandshakeMessages.encryptedExtensions ->
-  optCertRequest: option HandshakeMessages.certificateRequest13 ->
-  optServerCert: option Cert.chain13 -> // Not sent with PSK
-  optCertVerify: option HandshakeMessages.certificateVerify13 -> // Not sent with PSK
-  digest: option (b:bytes{length b <= 32}) ->
-  ST (result mode) // it needs to be computed, whether returned or not
-  (requires fun h0 -> 
-    inv ns h0 /\ (match HS.sel h0 ns.state with
-    | C_Mode m -> m.n_protocol_version = TLS_1p3
-    | _ -> False ))
-  (ensures fun h0 _ h1 -> True)
+  // optCertRequest: option HandshakeMessages.certificateRequest13 ->
+  sigdata: option (
+    Cert.chain13 * 
+    option HandshakeMessages.certificateVerify13 *
+    (b:bytes{length b <= 32})) ->
+  ST (result unit) // needs to be computed, whether returned or not
+  (requires fun h0 -> True)
+  (ensures fun h0 _ h1 -> B.modifies B.loc_none h0 h1)
   // [C_Mode ==> C_Complete] setting [sexts optCertRequest schain] in mode and recording [ccert]
   // ensures schain-based server authentication of the mode (including sexts) 
   // ensures consistency of sexts and schain with the offer.
@@ -434,6 +463,7 @@ val clientComplete_13:
 
 (* SERVER *) 
 
+(* 19-08-31 TODO get rid of stateful nego
 
 //17-03-30 still missing a few for servers.
 module HRR = Parsers.HelloRetryRequest
@@ -441,9 +471,6 @@ module HRR = Parsers.HelloRetryRequest
 noeq type serverMode =
   | ServerMode: mode -> certNego -> Extensions.unknownExtensions -> serverMode
   | ServerRetry: TLS.Cookie.(hrr_leq extensions_max_length) -> serverMode
-
-(* Returns the server hostName, if any, or an empty bytestring; review. *)
-val get_sni: offer -> Tot bytes 
 
 (* for QUIC *) 
 val get_alpn: offer -> Tot Extensions.clientHelloExtension_CHE_application_layer_protocol_negotiation
@@ -510,12 +537,11 @@ val server_ServerShare:
 
 
 
-
-
-
+*)
+ 
 //17-03-30 get rid of this wrapper?
 noeq type session = {
-  session_nego: option mode;
+  session_nego: option unit // mode;
 }
 
 /// Still used in Old.Epoch
@@ -529,6 +555,8 @@ noeq type handshake =
 // We tried using instead hs, but this creates circularities
 // We'll probably need a global log to reason about them.
 // We should probably do the same in the session store.
+
+
 
 
 /// QUIC uses ch accessors: 
