src/tls/Old.Epochs.fst
@@ -75,7 +75,7 @@ noeq type epoch (hs_rgn:rgn) (n:random) =
       epoch hs_rgn n
 
 // we would extend/adapt it for TLS 1.3,
-// e.g. to notify 0RTT/forwad-privacy transitions
+// e.g. to notify 0RTT/forward-privacy transitions
 // for now epoch completion is a total function on handshake --- should be stateful
 
 let epoch_id #r #n (e:epoch r n) : StAE.stae_id = Epoch?.i e
