src/tls/TLS.Handshake.Client.fsti
@@ -1,29 +1,33 @@
 module TLS.Handshake.Client
 
+/// Implementing the transitions of the Client state machine:
+/// processing incoming flights of messages, issuing messages, and
+/// advancing the key schedule.
+///
 open Mem
 open TLSConstants
 open TLSError
 open FStar.HyperStack.ST
-open TLS.Handshake.Machine
 
 module B = LowStar.Buffer // not FStar.Bytes
-module CH = Parsers.ClientHello
+module HS = FStar.HyperStack
 module HSM = HandshakeMessages
+module Nego = Negotiation
+module Hash = Hashing.Spec
 module HMAC = Old.HMAC.UFCMA
 module KS = Old.KeySchedule
-module HSL = HandshakeLog
-module Nego = Negotiation
-module HS = FStar.HyperStack
-module H = Hashing.Spec
+
+open TLS.Handshake.Machine
+
+// defined elsewhere?
+let inv (Client rgn cfg st:client) h0 =
+  h0 `HS.contains` st /\
+  B.loc_disjoint (B.loc_mreference st) (client_footprint (HS.sel h0 st)) /\
+  client_invariant (HS.sel h0 st) h0
 
 (*** Hello messages ***)
 
-let inv (Client rgn cfg st:client) h0 =
-  h0 `HS.contains` st /\
-  B.loc_disjoint (B.loc_mreference st) (TLS.Handshake.Machine.client_footprint (HS.sel h0 st)) /\
-  TLS.Handshake.Machine.client_invariant (HS.sel h0 st) h0
-
-/// C_Init ==> C_wait_ServerHello
+/// C_Init ==> C_wait_ServerHello (initial)
 val client_ClientHello:
   hs: client ->
   ST (result unit)
@@ -34,7 +38,6 @@ val client_ClientHello:
   (ensures fun h0 r h1 ->
     // see precise post-condition in the stateful invariant
     inv hs h1)
-
 (*
     let n = HS.sel h0 Nego.(s.nego.state) in
     let t = HSL.transcript h0 s.log in
@@ -57,6 +60,7 @@ val client_ClientHello:
         | _ -> False )))
 *)
 
+/// C_wait_ServerHello (initial) ==> C_wait_ServerHello (retried)
 val client_HelloRetryRequest:
   hs: client ->
   hrr: HSM.hrr ->
@@ -68,13 +72,7 @@ val client_HelloRetryRequest:
   (ensures fun h0 r h1 ->
     inv hs h1)
 
-(* useless?
-let client_sel_t (Client rgn cfg r:client) = client_state rgn cfg
-let client_sel h c: GTot (client_sel_t c) =
-  let Client rgn cfg r = c in
-  HS.sel h r
-*)
-
+/// C_wait_ServerHello (any) ==> C13_wait_Finished1
 val client_ServerHello:
   hs: client ->
   sh: HSM.sh ->
@@ -86,66 +84,46 @@ val client_ServerHello:
   (ensures fun h0 r h1 ->
     inv hs h1)
 
-
-val client_ServerHello_HRR:
-  hs: hs ->
-  ch1: Nego.offer ->
-  hrr: Nego.retryInfo ch1 ->
-  sh: HSM.sh ->
-  St incoming
-
-(*** TLS 1.2 ***)
-
-val client_ServerHelloDone:
-  hs: client ->
-  cert: HSM.certificate12 ->
-  ske_bytes: Bytes.bytes -> // delayed parsing
-  cr: option HSM.certificateRequest12 ->
-  ST Receive.incoming
-  (requires fun h0 -> inv hs h0)
-  (ensures fun h0 i h1 -> inv hs h1)
-
-val client_R_ServerFinished:
-  hs: client ->
-  f: Bytes.bytes ->
-  digest_nst: H.anyTag ->
-  digest_sf: H.anyTag ->
-  ST Receive.incoming
-  (requires fun h0 -> inv hs h0)
-  (ensures fun h0 i h1 -> inv hs h1)
-
-val client_ServerFinished:
-  hs: client ->
-  fin: Bytes.bytes ->
-  digest: H.anyTag ->
-  ST Receive.incoming
-  (requires fun h0 -> inv hs h0)
-  (ensures fun h0 i h1 -> inv hs h1)
-
-val client_NewSessionTicket_12:
-  hs: client ->
-  resume: bool ->
-  digest: H.anyTag ->
-  nst: HSM.newSessionTicket12 ->
-  ST Receive.incoming
-  (requires fun h0 -> inv hs h0)
-  (ensures fun h0 i h1 -> inv hs h1)
-
 (*** TLS 1.3 ***)
 
-/// process the TLS 1.3 decrypted server flight
-/// EncryptedExtension...ServerFinished
+/// Send the client second flight (typically just Finished) and
+/// conclude the handshake; this final step of client13_Finished1 may
+/// be delayed till the key change after EOED.
+
+// we may instead get cfk from ks
+// we may need to add ghost input and output transcripts
+
+val client13_Finished2:
+  hs: client ->
+  // cr: option HSM.certificateRequest13 ->
+  ST (result unit)
+  (requires fun h0 ->
+    let Client _ _ r = hs in
+    inv hs h0 /\
+    C13_complete? (HS.sel h0 r))
+  (ensures fun h0 r h1 ->
+    let Client _ _ r = hs in
+    inv hs h1 /\
+    C13_complete? (HS.sel h1 r) )
+
+/// C13_wait_Finished1 ==> C13_complete
 ///
-val c13_Finished1:
+/// process the TLS 1.3 decrypted server flight
+/// [EncryptedExtension..Finished1].
+///
+/// All these messages still require hashing
+///
+/// If successful, complete the key exchange and send [Finished2].
+///
+val client13_Finished1:
   hs: client ->
   ee: HSM.encryptedExtensions ->
   ocr: option HSM.certificateRequest13 ->
-  oc: option HSM.certificate13 ->
-  ocv: option HSM.certificateVerify13 ->
+  ocvv: option (HSM.certificate13 * HSM.certificateVerify13) ->
   svd: Bytes.bytes ->
-  digestCert: option H.anyTag ->
-  digestCertVerify: H.anyTag ->
-  digestServerFinished: H.anyTag ->
+  // digestCert: option Hash.anyTag ->
+  // digestCertVerify: Hash.anyTag ->
+  // digestServerFinished: Hash.anyTag ->
   ST Receive.incoming
   (requires fun h0 ->
     let Client _ _ r = hs in
@@ -153,15 +131,10 @@ val c13_Finished1:
     C13_wait_Finished1? (HS.sel h0 r))
   (ensures fun h0 i h1 -> inv hs h1)
 
-// Send ClientFinished flight (hide from API?)
-val client_ClientFinished_13:
-  hs: client ->
-  digest: H.anyTag ->
-  cr: option HSM.certificateRequest13 ->
-  cfk: (i:HMAC.finishedId & cfk:KS.fink i) ->
-  St unit
+/// Post-handshake incoming ticket
+/// (stays in C13_complete)
 
-val c13_NewSessionTicket:
+val client13_NewSessionTicket:
   hs: client ->
   nst: HSM.newSessionTicket13 ->
   ST Receive.incoming
@@ -171,9 +144,46 @@ val c13_NewSessionTicket:
     C13_complete? (HS.sel h0 r))
   (ensures fun h0 i h1 -> inv hs h1)
 
-// used for QUIC signalling; underspecified
+/// used for QUIC signalling; underspecified
 val early_rejected:
   hs: client ->
   ST bool
   (requires fun h0 -> inv hs h0)
   (ensures fun h0 r h1 -> h0 == h1)
+
+(*** TLS 1.2 ***)
+
+val client12_ServerHelloDone:
+  hs: client ->
+  cert: HSM.certificate12 ->
+  ske_bytes: Bytes.bytes -> // delayed parsing
+  cr: option HSM.certificateRequest12 ->
+  ST Receive.incoming
+  (requires fun h0 -> inv hs h0)
+  (ensures fun h0 i h1 -> inv hs h1)
+
+val client12_R_ServerFinished:
+  hs: client ->
+  f: Bytes.bytes ->
+  digest_nst: Hash.anyTag ->
+  digest_sf: Hash.anyTag ->
+  ST Receive.incoming
+  (requires fun h0 -> inv hs h0)
+  (ensures fun h0 i h1 -> inv hs h1)
+
+val client12_ServerFinished:
+  hs: client ->
+  fin: Bytes.bytes ->
+  digest: Hash.anyTag ->
+  ST Receive.incoming
+  (requires fun h0 -> inv hs h0)
+  (ensures fun h0 i h1 -> inv hs h1)
+
+val client12_NewSessionTicket:
+  hs: client ->
+  resume: bool ->
+  digest: Hash.anyTag ->
+  nst: HSM.newSessionTicket12 ->
+  ST Receive.incoming
+  (requires fun h0 -> inv hs h0)
+  (ensures fun h0 i h1 -> inv hs h1)
